spec/lean/Spec.lean
@@ -1,4 +1,5 @@
 import Spec.Lookup
 import Spec.LookupProofs
+import Spec.LookupProofsTimeout
 import Spec.Axioms
 import Spec.Address
